ADT: add kernel entry/exit constraints on domain time left
These changes to the automatons are required by:
  SELFOUR-242: invert bitfield scheduler and optimise fast path

Details:

When we enter the kernel, the domain time left (ksDomainTime) is never zero.
If we entered on a timer interrupt, we may decrement it to zero before the
scheduler runs. If we do so, we set the scheduler state to choose_new_thread.

When choosing a new thread, the scheduler switches to a new domain if the
present one is required, and sets the new domain time left from domain_list
(ksDomSchedule).

When entering the kernel on a non-interrupt event, we never touch the domain
time left, which trivially preserves the new constraints.

To prove these, we had to ban a transition from kernel entry to kernel being
preempted when handling an interrupt event in InfoFlow. This is fine, as by
design handling interrupts is not meant to be preempted by interrupts.

proof/infoflow/ADT_IF.thy
@@ -701,9 +701,11 @@ definition
   where
   "global_automaton_if get_active_irqf do_user_opf kernel_callf 
                        preemptionf schedulef kernel_exitf \<equiv>
-  (* Kernel entry with preemption during event handling *)
+  (* Kernel entry with preemption during event handling
+     NOTE: kernel cannot be preempted while servicing an interrupt *)
      { ( (s, KernelEntry e),
-         (s', KernelPreempted) ) |s s' e. (s, True, s') \<in> kernel_callf e } \<union>
+         (s', KernelPreempted) ) |s s' e. (s, True, s') \<in> kernel_callf e \<and>
+                                          e \<noteq> Interrupt} \<union>
   (* kernel entry without preemption during event handling *)
      { ( (s, KernelEntry e),
          (s', KernelSchedule (e = Interrupt)) ) |s s' e. (s, False, s') \<in> kernel_callf e } \<union>
@@ -1062,11 +1064,14 @@ lemma kernel_entry_if_guarded_pas_domain:
   done
 
 lemma kernel_entry_if_valid_sched:
-  "\<lbrace>valid_sched and invs and
+  "\<lbrace>valid_sched and invs and (ct_active or ct_idle) and
     (\<lambda>s. (e \<noteq> Interrupt \<longrightarrow> ct_active s) \<and> scheduler_action s = resume_cur_thread)\<rbrace>
    kernel_entry_if e tc
    \<lbrace>\<lambda>_. valid_sched\<rbrace>"
-  apply(simp add: kernel_entry_if_def tcb_cap_cases_def | wp static_imp_wp handle_event_valid_sched thread_set_invs_trivial thread_set_not_state_valid_sched)+
+  apply(simp add: kernel_entry_if_def tcb_cap_cases_def
+        | wp static_imp_wp handle_event_valid_sched thread_set_invs_trivial
+             thread_set_not_state_valid_sched hoare_vcg_disj_lift
+             thread_set_no_change_tcb_state ct_in_state_thread_state_lift)+
   apply(clarsimp)
   done
 
@@ -1376,23 +1381,30 @@ lemma valid_device_abs_state_eq:
 
 
 
+
 (*Weakened invs_if to properties only necessary for refinement*)
 definition full_invs_if :: "observable_if set" where
-  "full_invs_if \<equiv> {s. einvs (internal_state_if s) \<and>         
-                (case (snd s) of (KernelEntry e) \<Rightarrow>
-                     (e \<noteq> Interrupt \<longrightarrow> ct_running (internal_state_if s)) \<and>
-                     (ct_running (internal_state_if s) \<or> ct_idle (internal_state_if s)) \<and>
-                      
-                     scheduler_action (internal_state_if s) = resume_cur_thread
-                              | KernelExit \<Rightarrow>
-                     (ct_running (internal_state_if s) \<or> ct_idle (internal_state_if s)) \<and>
-                     scheduler_action (internal_state_if s) = resume_cur_thread                                          | InUserMode \<Rightarrow> 
-                     ct_running (internal_state_if s) \<and> 
-                     scheduler_action (internal_state_if s) = resume_cur_thread
-                              | InIdleMode \<Rightarrow> 
-                     ct_idle (internal_state_if s) \<and>
-                     scheduler_action (internal_state_if s) = resume_cur_thread
-                              | _ \<Rightarrow> True) }"
+  "full_invs_if \<equiv>
+    {s. einvs (internal_state_if s) \<and>
+        (snd s \<noteq> KernelSchedule True \<longrightarrow> domain_time (internal_state_if s) > 0) \<and>
+        (domain_time (internal_state_if s) = 0
+           \<longrightarrow> scheduler_action (internal_state_if s) = choose_new_thread) \<and>
+        valid_domain_list (internal_state_if s) \<and>
+        (case (snd s)
+          of (KernelEntry e) \<Rightarrow>
+                (e \<noteq> Interrupt \<longrightarrow> ct_running (internal_state_if s))
+                \<and> (ct_running (internal_state_if s) \<or> ct_idle (internal_state_if s))
+                \<and> scheduler_action (internal_state_if s) = resume_cur_thread
+           | KernelExit \<Rightarrow>
+                (ct_running (internal_state_if s) \<or> ct_idle (internal_state_if s))
+                \<and> scheduler_action (internal_state_if s) = resume_cur_thread
+           | InUserMode \<Rightarrow>
+                ct_running (internal_state_if s)
+                \<and> scheduler_action (internal_state_if s) = resume_cur_thread
+           | InIdleMode \<Rightarrow>
+                ct_idle (internal_state_if s)
+                \<and> scheduler_action (internal_state_if s) = resume_cur_thread
+           | _ \<Rightarrow> True) }"
 
 end
 
@@ -1500,16 +1512,6 @@ lemma ct_active_not_idle: "ct_active s \<Longrightarrow> invs s \<Longrightarrow
   apply (clarsimp simp add: ct_in_state_def valid_state_def valid_idle_def
                    pred_tcb_at_def obj_at_def invs_def)
   done
-
-(* it makes life easier to assume that all domain slies in the domain list are non-zero.
-   this means that when we switch to a new domain, the new domain_time is nonzero at least
-   until we get the first timer interrupt. this allows us to assume that we won't switch
-   partitions until at least after the first timer tick. *)
-definition valid_domain_list_2 where
-  "valid_domain_list_2 dl \<equiv> length dl > 0 \<and> (\<forall>(d,n) \<in> set dl. n > (0::word32))"
-
-abbreviation valid_domain_list where
-  "valid_domain_list s \<equiv> valid_domain_list_2 (domain_list s)"
 
 definition cur_context where "cur_context s = tcb_context (the (get_tcb (cur_thread s) s))"
 
@@ -1681,6 +1683,7 @@ lemma schedule_if_domain_time_nonzero':
    schedule_if tc
    \<lbrace>(\<lambda>_ s. domain_time s > 0)\<rbrace>"
   apply(simp add: schedule_if_def schedule_def)
+  apply (rule hoare_pre)
   apply (wp next_domain_domain_time_nonzero
         | wpc | simp add: crunch_simps guarded_switch_to_def switch_to_thread_def 
                               choose_thread_def switch_to_idle_thread_def
@@ -1688,11 +1691,9 @@ lemma schedule_if_domain_time_nonzero':
        apply(wp hoare_drop_imps)
         apply(simp add: choose_thread_def switch_to_idle_thread_def arch_switch_to_idle_thread_def guarded_switch_to_def switch_to_thread_def | wp)+
           apply(wp hoare_drop_imps)
+       apply clarsimp
        apply(wp next_domain_domain_time_nonzero)
-       apply simp
-     apply(wp_once hoare_drop_imps)
-     apply (wp)
-   apply clarsimp
+       apply (clarsimp simp: if_apply_def2)
   apply(wp gts_wp)
   apply (auto)
   done
@@ -2064,26 +2065,30 @@ definition cur_thread_context_of :: "observable_if \<Rightarrow> user_context" w
          | _ \<Rightarrow> cur_context (internal_state_if s)"
 
 definition invs_if :: "observable_if \<Rightarrow> bool" where
-  "invs_if s \<equiv> Invs (internal_state_if s) \<and>
-               det_inv (sys_mode_of s) (cur_thread_context_of s) (internal_state_if s) \<and>
-                (snd s \<noteq> KernelSchedule True \<longrightarrow> domain_time (internal_state_if s) > 0) \<and>
-                (domain_time (internal_state_if s) = 0 \<longrightarrow> scheduler_action (internal_state_if s) = choose_new_thread) \<and> (snd s \<noteq> KernelExit \<longrightarrow> (ct_idle (internal_state_if s) \<longrightarrow> 
-                            user_context_of s = idle_context (internal_state_if s))) \<and>
-                (case (snd s) of (KernelEntry e) \<Rightarrow>
+  "invs_if s \<equiv>
+    Invs (internal_state_if s) \<and>
+    det_inv (sys_mode_of s) (cur_thread_context_of s) (internal_state_if s) \<and>
+    (snd s \<noteq> KernelSchedule True \<longrightarrow> domain_time (internal_state_if s) > 0) \<and>
+    (domain_time (internal_state_if s) = 0
+       \<longrightarrow> scheduler_action (internal_state_if s) = choose_new_thread) \<and>
+    (snd s \<noteq> KernelExit
+       \<longrightarrow> (ct_idle (internal_state_if s)
+             \<longrightarrow> user_context_of s = idle_context (internal_state_if s))) \<and>
+    (case (snd s)
+      of KernelEntry e \<Rightarrow>
                      (e \<noteq> Interrupt \<longrightarrow> ct_running (internal_state_if s)) \<and>
                      (ct_running (internal_state_if s) \<or> ct_idle (internal_state_if s)) \<and>
-                      
                      scheduler_action (internal_state_if s) = resume_cur_thread
-                              | KernelExit \<Rightarrow>
+        | KernelExit \<Rightarrow>
                      (ct_running (internal_state_if s) \<or> ct_idle (internal_state_if s)) \<and>
-                     scheduler_action (internal_state_if s) = resume_cur_thread                                          | InUserMode \<Rightarrow> 
-                     ct_running (internal_state_if s) \<and> 
                      scheduler_action (internal_state_if s) = resume_cur_thread
-                              | InIdleMode \<Rightarrow> 
+        | InUserMode \<Rightarrow>
+                     ct_running (internal_state_if s) \<and>
+                     scheduler_action (internal_state_if s) = resume_cur_thread
+        | InIdleMode \<Rightarrow>
                      ct_idle (internal_state_if s) \<and>
                      scheduler_action (internal_state_if s) = resume_cur_thread
-                              | _ \<Rightarrow> True)"
-                       
+        | _ \<Rightarrow> True)"
 
 lemma invs_if_s0[simp]:
   "invs_if s0"
@@ -2307,6 +2312,7 @@ lemma invs_if_Step_ADT_A_if:
                      ct_idle_lift
                  | clarsimp intro: guarded_pas_is_subject_current_aag
                  | wp kernel_entry_if_domain_fields)+
+          apply (rule conjI, fastforce intro!: active_from_running)
           apply (simp add: schact_is_rct_def)
           apply (rule guarded_pas_is_subject_current_aag,assumption+)
          apply (simp_all only: silc_inv_cur pas_refined_cur guarded_pas_domain_cur)
@@ -2456,8 +2462,7 @@ lemma execution_restrict:
   done
 
 lemma invs_if_full_invs_if: "invs_if s \<Longrightarrow> s \<in> full_invs_if"
-  apply (clarsimp simp add: full_invs_if_def invs_if_def Invs_def)
-  done
+  by (clarsimp simp add: full_invs_if_def invs_if_def Invs_def)
 
 lemma ADT_A_if_Step_system:
   "Step_system (ADT_A_if utf) s0"
@@ -3397,12 +3402,16 @@ lemma ADT_A_if_Step_measure_if'':
   "\<lbrakk>(s,s') \<in> data_type.Step (ADT_A_if utf) x; invs_if s;
    measuref_if y s > 0\<rbrakk>
        \<Longrightarrow> measuref_if y s' < measuref_if y s \<and> 
-          (\<not> interrupted_modes (snd s) \<longrightarrow> interrupted_modes (snd s') \<longrightarrow> irq_state_of_state (internal_state_if s') = next_irq_state_of_state (internal_state_if s))"
+          (\<not> interrupted_modes (snd s) \<longrightarrow> interrupted_modes (snd s')
+            \<longrightarrow> irq_state_of_state (internal_state_if s') = next_irq_state_of_state (internal_state_if s))"
   apply(frule invs_if_irq_is_recurring)
   apply(case_tac s, clarsimp)
   apply(rename_tac uc i_s mode)
   apply(case_tac mode)
-       apply(simp_all add: rah_simp system.Step_def execution_def steps_def ADT_A_if_def global_automaton_if_def check_active_irq_A_if_def do_user_op_A_if_def check_active_irq_if_def in_monad measuref_if_def | safe | split if_splits)+
+       apply(simp_all add: rah_simp system.Step_def execution_def steps_def ADT_A_if_def
+                           global_automaton_if_def check_active_irq_A_if_def do_user_op_A_if_def
+                           check_active_irq_if_def in_monad measuref_if_def
+             | safe | split if_splits)+
                          apply(frule getActiveIRQ_None)
                          apply(erule use_valid[OF _ do_user_op_if_irq_measure_if])
                          apply(erule use_valid[OF _ dmo_getActiveIRQ_wp])
@@ -3439,13 +3448,15 @@ lemma ADT_A_if_Step_measure_if'':
                  apply(simp add: next_irq_state_Suc recurring_next_irq_state_dom)
                  apply(fastforce dest: next_irq_state_less)
                 apply(clarsimp split: if_splits)
-               apply(clarsimp split: if_splits)
-               apply(clarsimp simp: kernel_call_A_if_def kernel_entry_if_def in_monad)
-              apply (clarsimp simp: kernel_call_A_if_def)
-              apply (case_tac r,simp)
+                
+               apply(clarsimp simp: kernel_call_A_if_def in_monad)
+               apply (case_tac r ; simp)
                apply (rule kernel_entry_if_next_irq_state_of_state_next,assumption+)
-                  apply((simp add: invs_if_def Invs_def only_timer_irq_inv_def | elim conjE | assumption)+)[5]
-             apply(clarsimp split: if_splits)
+                  prefer 4
+                  apply fastforce
+                 apply((simp add: invs_if_def Invs_def only_timer_irq_inv_def | elim conjE | assumption)+)[3]
+              apply(clarsimp split: if_splits)
+
             apply(rule Suc_le_lessD)           
             apply simp
             apply(simp add: kernel_call_A_if_def)
