proof/crefine/Refine_C.thy
@@ -485,11 +485,11 @@ lemma ccorres_corres_u_xf:
 definition
   "all_invs' e \<equiv> \<lambda>s'. \<exists>s :: det_state.
     (s,s') \<in> state_relation \<and>
-    (einvs s \<and> (e \<noteq> Interrupt \<longrightarrow> ct_running s) \<and>
-      scheduler_action s = resume_cur_thread) \<and>
+    (einvs s \<and> (e \<noteq> Interrupt \<longrightarrow> ct_running s) \<and> (ct_running s \<or> ct_idle s) \<and>
+      scheduler_action s = resume_cur_thread \<and> domain_time s \<noteq> 0) \<and>
     (invs' s' \<and> vs_valid_duplicates' (ksPSpace s') \<and>
-      (e \<noteq> Interrupt \<longrightarrow> ct_running' s') \<and>
-      ksSchedulerAction s' = ResumeCurrentThread)"
+      (e \<noteq> Interrupt \<longrightarrow> ct_running' s') \<and> (ct_running' s' \<or> ct_idle' s') \<and>
+      ksSchedulerAction s' = ResumeCurrentThread  \<and> ksDomainTime s' \<noteq> 0)"
 
 lemma no_fail_callKernel:
   "no_fail (all_invs' e) (callKernel e)"
@@ -577,6 +577,13 @@ lemma ccorres_get_registers:
                         "StrictC'_register_defs")
   done
 
+(* FIXME: move *)
+lemma st_tcb_at'_opeq_simp:
+  "st_tcb_at' (op = Structures_H.thread_state.Running) (ksCurThread s) s
+    = st_tcb_at' (\<lambda>st. st = Structures_H.thread_state.Running) (ksCurThread s) s"
+  by (fastforce simp add: st_tcb_at'_def obj_at'_def)
+
+
 lemma callKernel_withFastpath_corres_C:
   "corres_underlying rf_sr False True dc
            (all_invs' e)
@@ -603,7 +610,9 @@ lemma callKernel_withFastpath_corres_C:
   apply (clarsimp simp: all_invs'_def rf_sr_ksCurThread)
   apply (frule(1) obj_at_cslift_tcb[OF tcb_at_invs'])
   apply (clarsimp simp: typ_heap_simps' ct_in_state'_def
-                        "StrictC'_register_defs" word_sle_def word_sless_def)
+                        "StrictC'_register_defs" word_sle_def word_sless_def
+                        st_tcb_at'_opeq_simp)
+  apply (rule conjI, fastforce simp: st_tcb_at'_def)
   apply (auto elim!: pred_tcb'_weakenE cnode_caps_gsCNodes_from_sr[rotated])
   done
 
@@ -620,7 +629,10 @@ lemma threadSet_all_invs_triv':
      apply (simp add: exst_same_def)
     apply (wp thread_set_invs_trivial thread_set_ct_running thread_set_not_state_valid_sched
               threadSet_invs_trivial threadSet_ct_running' static_imp_wp
-           | simp add: tcb_cap_cases_def)+
+              thread_set_ct_idle
+           | simp add: tcb_cap_cases_def
+           | rule threadSet_ct_in_state'
+           | wp_once hoare_vcg_disj_lift)+
   apply clarsimp
   apply (rule exI, rule conjI, assumption)
   apply (clarsimp simp: invs_def invs'_def cur_tcb_def cur_tcb'_def)
@@ -935,28 +947,6 @@ lemma do_user_op_corres_C:
    apply clarsimp
   done
 
-lemma checkActiveIRQ_ex_abs_einvs:
-  "\<lbrace>invs' and ex_abs einvs and (\<lambda>s. vs_valid_duplicates' (ksPSpace s)) and (ct_running' or ct_idle')
-    and (\<lambda>s. ksSchedulerAction s = ResumeCurrentThread)\<rbrace>
-   checkActiveIRQ
-   \<lbrace>\<lambda>_. ex_abs einvs\<rbrace>"  
-  apply (rule hoare_name_pre_state)
-  apply (simp add: ex_abs_def)
-  apply (rule_tac Q="\<lambda>r' s'. \<exists>r s. (s, s') \<in> state_relation \<and> einvs s \<and> dc r r'" in hoare_post_imp)
-   apply simp
-  apply (rule hoare_pre)
-  apply (rule valid_corres_combined[where Q'="\<lambda>x y. True", simplified, where rr=dc and sr=state_relation and f="check_active_irq"])
-  apply (rule hoare_post_imp[OF _ check_active_irq_invs], clarsimp)
-  apply (rule corres_rel_imp)
-  apply (rule corres_guard_imp[OF check_active_irq_corres])
-  apply (force simp: sched_act_rct_related)
-  apply simp
-  apply (simp add: hoare_TrueI)+
-  apply clarsimp
-  apply (rule_tac x=sb in exI)
-  apply (fastforce simp: ct_running_related ct_idle_related sched_act_rct_related)
-  done
-
 lemma check_active_irq_corres_C:
   "corres_underlying rf_sr False True (op =)
              (invs' and (\<lambda>s. ksSchedulerAction s = ResumeCurrentThread) and ex_abs valid_state) \<top>
@@ -985,6 +975,7 @@ lemma refinement2_both:
   "\<lparr> Init = Init_C, Fin = Fin_C,
      Step = (\<lambda>u. global_automaton check_active_irq_C (do_user_op_C uop) (kernel_call_C fp)) \<rparr>
    \<sqsubseteq> ADT_H uop"
+  supply word_neq_0_conv[simp]
   apply (rule sim_imp_refines)
   apply (rule L_invariantI [where I\<^sub>c=UNIV and r="lift_state_relation rf_sr"])
     apply (rule full_invs_both)
@@ -1021,8 +1012,7 @@ lemma refinement2_both:
           simp add: sch_act_simple_def)
     apply (fastforce simp: ct_running'_C)
     apply (clarsimp simp: full_invs_def full_invs'_def all_invs'_def)
-   apply (rule_tac x=bf in exI)
-   apply simp
+   apply fastforce
 
   apply (erule_tac P="a \<and> b \<and> c \<and> d \<and> e" for a b c d e in disjE)
    apply (clarsimp simp add: do_user_op_C_def do_user_op_H_def monad_to_transition_def)
