proof/invariant-abstract/DetSchedDomainTime_AI.thy
@@ -1,0 +1,414 @@
+(*
+ * Copyright 2014, General Dynamics C4 Systems
+ *
+ * This software may be distributed and modified according to the terms of
+ * the GNU General Public License version 2. Note that NO WARRANTY is provided.
+ * See "LICENSE_GPLv2.txt" for details.
+ *
+ * @TAG(GD_GPL)
+ *)
+
+theory DetSchedDomainTime_AI
+imports "$L4V_ARCH/ArchDetSchedAux_AI"
+begin
+
+text {*
+  This theory deals with the preservation of domain_list validity over kernel invocations,
+  as well as ensuring preserving that the domain time is never zero at kernel exit.
+*}
+
+(* Note: domains in the domain list should also be \<le> maxDomain, but this is not needed right now *)
+definition
+  "valid_domain_list_2 dlist \<equiv> 0 < length dlist \<and> (\<forall>(d,time) \<in> set dlist. 0 < time)"
+
+abbreviation
+  valid_domain_list :: "det_ext state \<Rightarrow> bool"
+where
+  "valid_domain_list \<equiv> (\<lambda>s. valid_domain_list_2 (domain_list s))"
+
+lemmas valid_domain_list_def = valid_domain_list_2_def
+
+
+section {* Preservation of domain list validity *}
+
+lemma ethread_get_wp[wp]:
+  "\<lbrace>\<lambda>s. etcb_at (\<lambda>t. P (f t) s) ptr s\<rbrace> ethread_get f ptr \<lbrace>P\<rbrace>"
+  unfolding ethread_get_def
+  by (wp | clarsimp simp add: get_etcb_def etcb_at'_def is_etcb_at'_def)+
+
+crunch domain_list_inv[wp]:
+  cap_swap_for_delete, empty_slot, get_object, get_cap, tcb_sched_action
+  "\<lambda>s. P (domain_list s)"
+
+context begin interpretation Arch . (*FIXME: arch_split*)
+
+crunch domain_list_inv[wp]: finalise_cap "\<lambda>s. P (domain_list s)"
+  (wp: crunch_wps hoare_drop_imps hoare_unless_wp select_inv mapM_wp
+       subset_refl if_fun_split simp: crunch_simps ignore: tcb_sched_action)
+
+lemma rec_del_domain_list[wp]:
+  "\<lbrace>\<lambda>s. P (domain_list s)\<rbrace> rec_del call \<lbrace>\<lambda>rv s. P (domain_list s)\<rbrace>"
+  by (wp rec_del_preservation preemption_point_inv' | simp)+
+
+crunch domain_list_inv[wp]: cap_delete, activate_thread "\<lambda>s. P (domain_list s)"
+
+crunch domain_list_inv[wp]: schedule "\<lambda>s. P (domain_list s)"
+  (wp: hoare_drop_imp simp: Let_def)
+
+end
+
+crunch domain_list_inv[wp]: handle_interrupt "\<lambda>s. P (domain_list s)"
+
+crunch domain_list_inv[wp]:
+  lookup_cap_and_slot, cap_insert, set_extra_badge "\<lambda>s. P (domain_list s)"
+  (wp: hoare_drop_imps)
+
+crunch domain_list_inv[wp]: do_ipc_transfer "\<lambda>s. P (domain_list s)"
+  (wp: crunch_wps transfer_caps_loop_pres simp: zipWithM_x_mapM ignore: transfer_caps_loop)
+
+crunch domain_list_inv[wp]: copy_mrs "\<lambda>s. P (domain_list s)"
+
+crunch domain_list_inv[wp]: handle_fault "\<lambda>s. P (domain_list s)"
+  (wp: mapM_wp hoare_drop_imps simp: crunch_simps ignore:copy_mrs)
+
+crunch domain_list_inv[wp]:
+  reply_from_kernel, create_cap, retype_region, do_reply_transfer
+  "\<lambda>s. P (domain_list s)"
+  (wp: hoare_drop_imps)
+
+crunch domain_list_inv[wp]: delete_objects "\<lambda>s :: det_ext state. P (domain_list s)"
+  (wp: crunch_wps
+   simp: detype_def detype_ext_def wrap_ext_det_ext_ext_def cap_insert_ext_def
+   ignore: freeMemory)
+
+crunch domain_list_inv[wp]: update_work_units "\<lambda>s. P (domain_list s)"
+
+crunch domain_list_inv[wp]: preemption_point "\<lambda>s. P (domain_list s)"
+  (wp: select_inv OR_choiceE_weak_wp ignore: OR_choiceE)
+
+crunch domain_list_inv[wp]: reset_untyped_cap "\<lambda>s. P (domain_list s)"
+  (wp: crunch_wps hoare_unless_wp mapME_x_inv_wp select_inv
+   simp: crunch_simps)
+
+context begin interpretation Arch . (*FIXME: arch_split*)
+
+crunch domain_list_inv[wp]: invoke_untyped "\<lambda>s. P (domain_list s)"
+  (wp: crunch_wps
+    simp: crunch_simps mapM_x_defsym)
+
+crunch domain_list_inv[wp]:
+  invoke_tcb, invoke_domain, invoke_irq_control, invoke_irq_handler
+  "\<lambda>s. P (domain_list s)"
+  (wp: crunch_wps check_cap_inv)
+
+crunch domain_list_inv[wp]: arch_perform_invocation "\<lambda>s. P (domain_list s)"
+  (wp: crunch_wps check_cap_inv)
+
+end
+
+crunch domain_list_inv[wp]: cap_move "\<lambda>s. P (domain_list s)"
+
+lemma cap_revoke_domain_list_inv[wp]:
+  "\<lbrace>(\<lambda>s :: det_ext state. P (domain_list s))\<rbrace> cap_revoke a \<lbrace>\<lambda>rv s. P (domain_list s)\<rbrace>"
+  by (rule cap_revoke_preservation2)
+     (wp preemption_point_inv'|simp)+
+
+crunch domain_list_inv[wp]: recycle_cap_ext "\<lambda>s. P (domain_list s)"
+
+context begin interpretation Arch . (*FIXME: arch_split*)
+
+crunch domain_list_inv[wp]: arch_recycle_cap "\<lambda>s. P (domain_list s)"
+  (ignore: filterM clearMemory recycle_cap_ext
+     simp: filterM_mapM crunch_simps
+       wp: crunch_wps hoare_unless_wp)
+
+end
+
+crunch domain_list_inv[wp]: recycle_cap "\<lambda>s. P (domain_list s)"
+  (ignore: filterM clearMemory recycle_cap_ext
+     simp: filterM_mapM crunch_simps
+       wp: crunch_wps)
+
+crunch domain_list_inv[wp]: cap_recycle "\<lambda>s. P (domain_list s)"
+  (wp: crunch_wps preemption_point_inv'
+   simp: crunch_simps filterM_mapM unless_def
+   ignore: without_preemption filterM recycle_cap_ext)
+
+lemma invoke_cnode_domain_list_inv[wp]:
+  "\<lbrace>\<lambda>s :: det_ext state. P (domain_list s)\<rbrace>
+     invoke_cnode i
+   \<lbrace>\<lambda>rv s. P (domain_list s) \<rbrace>"
+  apply (rule hoare_pre)
+   apply (wp crunch_wps cap_move_src_slot_Null hoare_drop_imps hoare_vcg_all_lift
+          | wpc | simp add: invoke_cnode_def crunch_simps split del: split_if)+
+  done
+
+crunch domain_list_inv[wp]: perform_invocation, handle_invocation "\<lambda>s. P (domain_list s)"
+  (wp: crunch_wps syscall_valid simp: crunch_simps ignore: without_preemption)
+
+context begin interpretation Arch . (*FIXME: arch_split*)
+
+crunch domain_list_inv[wp]:
+  handle_recv, handle_yield, handle_call, handle_reply, handle_vm_fault
+    "\<lambda>s. P (domain_list s)"
+  (wp: crunch_wps simp: crunch_simps)
+
+end
+
+lemma handle_event_domain_list_inv[wp]:
+  "\<lbrace>\<lambda>s. P (domain_list s) \<rbrace>
+   handle_event e
+   \<lbrace>\<lambda>_ s. P (domain_list s) \<rbrace>"
+  apply (cases e, simp_all)
+      apply (rename_tac syscall)
+      apply (case_tac syscall, simp_all add: handle_send_def)
+             apply (wp|simp|wpc)+
+  done
+
+(* no one modifies domain_list - supplied at compile time *)
+lemma call_kernel_domain_list_inv_det_ext:
+  "\<lbrace> \<lambda>s. P (domain_list s) \<rbrace>
+     (call_kernel e) :: (unit,det_ext) s_monad
+   \<lbrace>\<lambda>_ s. P (domain_list s) \<rbrace>"
+  unfolding call_kernel_def
+  apply (wp)
+   apply (simp add: schedule_def)
+   apply (wp without_preemption_wp|wpc|simp add: if_apply_def2)+
+  done
+
+
+section {* Preservation of domain time remaining *}
+
+crunch domain_time_inv[wp]: do_user_op "(\<lambda>s. P (domain_time s))"
+  (wp: select_wp)
+
+context begin interpretation Arch . (*FIXME: arch_split*)
+
+crunch domain_time_inv[wp]:
+  get_cap, activate_thread, set_scheduler_action, tcb_sched_action
+  "\<lambda>s. P (domain_time s)"
+
+crunch domain_time_inv[wp]: guarded_switch_to "\<lambda>s. P (domain_time s)"
+  (wp: hoare_drop_imp whenE_inv)
+
+crunch domain_time_inv[wp]: choose_thread "\<lambda>s. P (domain_time s)"
+
+end
+
+crunch domain_time_inv[wp]: send_signal "\<lambda>s. P (domain_time s)"
+  (wp: hoare_drop_imps mapM_x_wp_inv select_wp simp: crunch_simps unless_def)
+
+crunch domain_time_inv[wp]:
+  cap_swap_for_delete, empty_slot, get_object, get_cap, tcb_sched_action
+  "\<lambda>s. P (domain_time s)"
+
+context begin interpretation Arch . (*FIXME: arch_split*)
+
+crunch domain_time_inv[wp]: finalise_cap "\<lambda>s. P (domain_time s)"
+  (wp: crunch_wps hoare_drop_imps hoare_unless_wp select_inv mapM_wp
+       subset_refl if_fun_split simp: crunch_simps ignore: tcb_sched_action)
+
+end
+
+lemma rec_del_domain_time[wp]:
+  "\<lbrace>\<lambda>s. P (domain_time s)\<rbrace> rec_del call \<lbrace>\<lambda>rv s. P (domain_time s)\<rbrace>"
+  by (wp rec_del_preservation preemption_point_inv' | simp)+
+
+crunch domain_time_inv[wp]:
+  cap_delete, activate_thread, lookup_cap_and_slot
+  "\<lambda>s. P (domain_time s)"
+
+crunch domain_time_inv[wp]: cap_insert "\<lambda>s. P (domain_time s)"
+  (wp: hoare_drop_imps)
+
+crunch domain_time_inv[wp]: set_extra_badge "\<lambda>s. P (domain_time s)"
+
+crunch domain_time_inv[wp]: do_ipc_transfer "\<lambda>s. P (domain_time s)"
+  (wp: crunch_wps transfer_caps_loop_pres simp: zipWithM_x_mapM ignore: transfer_caps_loop)
+
+crunch domain_time_inv[wp]: copy_mrs "\<lambda>s. P (domain_time s)"
+
+crunch domain_time_inv[wp]: handle_fault "\<lambda>s. P (domain_time s)"
+  (wp: mapM_wp hoare_drop_imps simp: crunch_simps ignore:copy_mrs) 
+
+crunch domain_time_inv[wp]:
+  reply_from_kernel, create_cap, retype_region
+  "\<lambda>s. P (domain_time s)"
+
+crunch domain_time_inv[wp]: do_reply_transfer "\<lambda>s. P (domain_time s)"
+  (wp: hoare_drop_imps)
+
+crunch domain_time_inv[wp]: delete_objects "\<lambda>s :: det_ext state. P (domain_time s)"
+  (wp: crunch_wps
+   simp: detype_def detype_ext_def wrap_ext_det_ext_ext_def cap_insert_ext_def
+   ignore: freeMemory)
+
+crunch domain_time_inv[wp]: update_work_units "\<lambda>s. P (domain_time s)"
+
+crunch domain_time_inv[wp]: preemption_point "\<lambda>s. P (domain_time s)"
+  (wp: select_inv OR_choiceE_weak_wp ignore: OR_choiceE)
+
+crunch domain_time_inv[wp]: reset_untyped_cap "\<lambda>s. P (domain_time s)"
+  (wp: crunch_wps hoare_unless_wp mapME_x_inv_wp select_inv
+   simp: crunch_simps)
+
+context begin interpretation Arch . (*FIXME: arch_split*)
+
+crunch domain_time_inv[wp]: invoke_untyped "\<lambda>s. P (domain_time s)"
+  (wp: crunch_wps
+    simp: crunch_simps mapM_x_defsym)
+
+crunch domain_time_inv[wp]:
+  invoke_tcb, invoke_domain, invoke_irq_control,invoke_irq_handler
+  "\<lambda>s. P (domain_time s)"
+  (wp: crunch_wps check_cap_inv)
+
+crunch domain_time_inv[wp]: arch_perform_invocation "\<lambda>s. P (domain_time s)"
+  (wp: crunch_wps check_cap_inv)
+
+end
+
+crunch domain_time_inv[wp]: cap_move "\<lambda>s. P (domain_time s)"
+
+lemma cap_revoke_domain_time_inv[wp]:
+  "\<lbrace>(\<lambda>s :: det_ext state. P (domain_time s))\<rbrace> cap_revoke a \<lbrace>\<lambda>rv s. P (domain_time s)\<rbrace>"
+  apply (rule cap_revoke_preservation2)
+  apply (wp preemption_point_inv'|simp)+
+  done
+
+crunch domain_time_inv[wp]: recycle_cap_ext "\<lambda>s. P (domain_time s)"
+
+context begin interpretation Arch . (*FIXME: arch_split*)
+
+crunch domain_time_inv[wp]: arch_recycle_cap "\<lambda>s. P (domain_time s)"
+  (ignore: filterM clearMemory recycle_cap_ext
+     simp: filterM_mapM crunch_simps
+       wp: crunch_wps hoare_unless_wp)
+
+end
+
+crunch domain_time_inv[wp]: recycle_cap "\<lambda>s. P (domain_time s)"
+  (ignore: filterM clearMemory recycle_cap_ext
+     simp: filterM_mapM crunch_simps
+       wp: crunch_wps)
+
+crunch domain_time_inv[wp]: cap_recycle "\<lambda>s. P (domain_time s)"
+  (wp: crunch_wps preemption_point_inv'
+   simp: crunch_simps filterM_mapM unless_def
+   ignore: without_preemption filterM recycle_cap_ext)
+
+lemma invoke_cnode_domain_time_inv[wp]:
+  "\<lbrace>\<lambda>s :: det_ext state. P (domain_time s)\<rbrace>
+     invoke_cnode i
+   \<lbrace>\<lambda>rv s. P (domain_time s) \<rbrace>"
+  apply (rule hoare_pre)
+   apply (wp crunch_wps cap_move_src_slot_Null hoare_drop_imps hoare_vcg_all_lift
+          | wpc | simp add: invoke_cnode_def crunch_simps split del: split_if)+
+  done
+
+crunch domain_time_inv[wp]: perform_invocation, handle_invocation "\<lambda>s. P (domain_time s)"
+  (wp: crunch_wps syscall_valid simp: crunch_simps ignore: without_preemption)
+
+context begin interpretation Arch . (*FIXME: arch_split*)
+
+crunch domain_time_inv[wp]:
+  handle_recv, handle_yield, handle_call, handle_reply, handle_vm_fault
+    "\<lambda>s. P (domain_time s)"
+  (wp: crunch_wps simp: crunch_simps)
+
+end
+
+lemma handle_event_domain_time_inv:
+  "\<lbrace>\<lambda>s. P (domain_time s) \<and> e \<noteq> Interrupt \<rbrace>
+   handle_event e
+   \<lbrace>\<lambda>_ s. P (domain_time s) \<rbrace>"
+  apply (cases e, simp_all)
+      apply (rename_tac syscall)
+      apply (case_tac syscall, simp_all add: handle_send_def)
+             apply (wp|simp|wpc)+
+  done
+
+crunch domain_time_inv[wp]: send_fault_ipc, handle_call "\<lambda>s. P (domain_time s)"
+  (wp: hoare_drop_imps mapM_x_wp_inv select_wp without_preemption_wp simp: crunch_simps unless_def)
+
+lemma next_domain_domain_time_left[wp]:
+  "\<lbrace> valid_domain_list \<rbrace> next_domain \<lbrace>\<lambda>_ s. 0 < domain_time s \<rbrace>"
+  apply (rule hoare_pre)
+   apply (simp add: next_domain_def Let_def)
+    apply wp
+   apply (clarsimp simp: valid_domain_list_def)
+   apply (simp add: all_set_conv_all_nth)
+   apply (erule_tac x="Suc (domain_index s) mod length (domain_list s)" in allE)
+   apply clarsimp
+   done
+
+lemma schedule_domain_time_left:
+  "\<lbrace>valid_domain_list and (\<lambda>s. domain_time s = 0 \<longrightarrow> scheduler_action s = choose_new_thread) \<rbrace>
+   schedule
+   \<lbrace>\<lambda>_ s. 0 < domain_time s \<rbrace>" (is "\<lbrace>?P\<rbrace> _ \<lbrace>_\<rbrace>")
+  supply word_neq_0_conv[simp]
+  apply (simp add: schedule_def)
+  apply (wp|wpc)+
+     apply (rule_tac Q="\<lambda>_. valid_domain_list" in hoare_post_imp, fastforce)
+     apply wp
+   apply (rule_tac Q="\<lambda>_. ?P" in hoare_post_imp, fastforce)
+   apply wp
+  done
+
+lemma reschedule_required_valid_domain_time:
+  "\<lbrace> \<top> \<rbrace> reschedule_required
+   \<lbrace>\<lambda>x s. domain_time s = 0 \<longrightarrow> scheduler_action s = choose_new_thread\<rbrace>"
+  unfolding reschedule_required_def set_scheduler_action_def
+  by (wp hoare_vcg_imp_lift | simp | wpc)+
+
+(* FIXME: move to where hoare_drop_imp is, add E/R variants etc *)
+lemma hoare_false_imp:
+  "\<lbrace>P\<rbrace> f \<lbrace>\<lambda>r s. \<not> R r s\<rbrace> \<Longrightarrow> \<lbrace>P\<rbrace> f \<lbrace>\<lambda>r s. R r s \<longrightarrow> Q r s\<rbrace>"
+  by (auto simp: valid_def)
+
+context begin interpretation Arch . (*FIXME: arch_split*)
+
+lemma handle_interrupt_valid_domain_time:
+  "\<lbrace>\<lambda>s :: det_ext state. 0 < domain_time s \<rbrace> handle_interrupt i
+   \<lbrace>\<lambda>rv s.  domain_time s = 0 \<longrightarrow> scheduler_action s = choose_new_thread \<rbrace>"
+   apply (unfold handle_interrupt_def)
+   apply (case_tac "maxIRQ < i"; simp)
+    subgoal by (wp hoare_false_imp, simp)
+   apply (rule hoare_pre)
+    apply (wp do_machine_op_exst | simp | wpc)+
+       apply (rule_tac Q="\<lambda>_ s. 0 < domain_time s" in hoare_post_imp, fastforce)
+       apply wp
+      apply (rule_tac Q="\<lambda>_ s. 0 < domain_time s" in hoare_post_imp, fastforce)
+      apply wp
+     apply simp (* dxo_eq *)
+     apply (clarsimp simp: timer_tick_def num_domains_def)
+     apply (wp reschedule_required_valid_domain_time | simp | wp_once hoare_drop_imp)+
+   done
+
+end
+
+lemma call_kernel_domain_time_inv_det_ext:
+  "\<lbrace> (\<lambda>s. 0 < domain_time s) and valid_domain_list and (\<lambda>s. e \<noteq> Interrupt \<longrightarrow> ct_running s) \<rbrace>
+   (call_kernel e) :: (unit,det_ext) s_monad
+   \<lbrace>\<lambda>_ s. 0 < domain_time s \<rbrace>"
+  unfolding call_kernel_def
+  apply (case_tac "e = Interrupt")
+   apply simp
+   apply (rule hoare_pre)
+   apply ((wp schedule_domain_time_left handle_interrupt_valid_domain_time
+           | wpc | simp)+)[1]
+   apply (rule_tac Q="\<lambda>_ s. 0 < domain_time s \<and> valid_domain_list s" in hoare_strengthen_post)
+    apply wp
+   apply fastforce+
+  (* now non-interrupt case; may throw but does not touch domain_time in handle_event *)
+  apply (rule hoare_pre)
+   apply (wp schedule_domain_time_left without_preemption_wp handle_interrupt_valid_domain_time)
+    apply (rule_tac Q="\<lambda>_ s. 0 < domain_time s \<and> valid_domain_list s" in hoare_post_imp)
+     apply fastforce
+    apply (wp handle_event_domain_time_inv)
+   apply (rule_tac Q'="\<lambda>_ s. 0 < domain_time s" in hoare_post_imp_R)
+    apply (wp handle_event_domain_time_inv)
+   apply fastforce+
+  done
+
+end
