spec/abstract/Deterministic_A.thy
@@ -573,7 +573,7 @@ definition "ext_init_det_ext_ext \<equiv>
      \<lparr>work_units_completed_internal = 0,
       scheduler_action_internal = resume_cur_thread,
       ekheap_internal = Map.empty (idle_thread_ptr \<mapsto> default_etcb),
-      domain_list_internal = [],
+      domain_list_internal = [(0,15)],
       domain_index_internal = 0,
       cur_domain_internal = 0,
       domain_time_internal = 15,
